Filesys/PathBasedFSInv.i.dfy
@@ -8,22 +8,20 @@ module PathBasedFSInv {
   import opened FSTypes
   import opened PathSpec
 
-  // redirect meta should have no corresponding data entry ==> emptydata
-
+  // redirect meta should have no corresponding data entry ==> emptydata  
   predicate Inv(fs: FileSys)
   {
     && WF(fs)
-    // consistency of hidden map
-    // && (forall p | fs.hidden.meta_map[p].)
-
-
-    // path is connected
-    // && (forall path | PathExists(fs, path) && path != RootDir :: ParentDirIsDir(fs, path))
-    // redirect meta points to a valid and hidden path meta
-    // && (forall path | fs.meta_map[path].RedirectMeta? :: 
-    //     && fs.meta_map[fs.meta_map[path].source].PathMeta?
-    //     && fs.meta_map[fs.meta_map[path].source].hidden
-    //     && !fs.meta_map[fs.meta_map[path].source].m.ftype.Directory?)
+    // Note(Jialin): why need this one here again?
+    && (forall path | PathExists(fs, path) && path != RootDir :: ParentDirIsDir(fs, path))
+    // Hidden view consistency: no redirect in the hidden map
+    && (forall path :: !fs.hidden.meta_map[path].RedirectMeta?)
+    // Hidden view consistency: no directory in hidden map
+    && (forall path | fs.hidden.meta_map[path].MetaData? :: !fs.hidden.meta_map[path].ftype.Directory?)
+    // Content view and hidden view consistency: a redirect meta has a valid entry in hidden view
+    && (forall path | fs.content.meta_map[path].RedirectMeta? :: ValidHiddenEntry(fs, path))
+    // Content view and hidden view consistency: no dangly hidden view entries
+    && (forall hidden | fs.hidden.meta_map[hidden].MetaData? :: HasReference(fs, hidden))
   }
 
   lemma InitImpliesInv(fs: FileSys)
@@ -32,255 +30,176 @@ module PathBasedFSInv {
   {
   }
 
-  // lemma NextPreservesInv(fs: FileSys, fs': FileSys)
-  // requires Inv(fs)
-  // requires Next(fs, fs')
-  // ensures Inv(fs')
-  // {
-  //   var step :| NextStep(fs, fs', step);
-  //   NextStepPreservesInv(fs, fs', step);
-  // }
+  lemma NextPreservesInv(fs: FileSys, fs': FileSys)
+  requires Inv(fs)
+  requires Next(fs, fs')
+  ensures Inv(fs')
+  {
+    var step :| NextStep(fs, fs', step);
+    NextStepPreservesInv(fs, fs', step);
+  }
 
-  // lemma NextStepPreservesInv(fs: FileSys, fs': FileSys, step: Step)
-  // requires Inv(fs)
-  // requires NextStep(fs, fs', step)
-  // ensures Inv(fs')
-  // {
-  //   match step {
-  //     case DeleteStep(path, ctime) => DeletePreservesInv(fs, fs', path, ctime);
-  //     case RenameStep(source, dest, ctime) => RenamePreservesInv(fs, fs', source, dest, ctime);
-  //     case LinkStep(source, dest, ctime, hiddenName) => LinkPreservesInv(fs, fs', source, dest, ctime, hiddenName);
-  //     case _ => {
-  //       if step.CreateStep? || step.ChangeAttrStep? || step.TruncateStep? || step.WriteStep? || step.UpdateTimeStep? {
-  //         SimpleStepPreservesInv(fs, fs', step);
-  //       }
-  //     }
-  //   }
-  // }
+  lemma NextStepPreservesInv(fs: FileSys, fs': FileSys, step: Step)
+  requires Inv(fs)
+  requires NextStep(fs, fs', step)
+  ensures Inv(fs')
+  {
+    match step {
+      case DeleteStep(path, ctime) => DeletePreservesInv(fs, fs', path, ctime);
+      case RenameStep(source, dest, ctime) => RenamePreservesInv(fs, fs', source, dest, ctime);
+      case LinkStep(source, dest, ctime, hiddenName) => LinkPreservesInv(fs, fs', source, dest, ctime, hiddenName);
+      case _ => {
+        if step.CreateStep? || step.ChangeAttrStep? || step.TruncateStep? || step.WriteStep? || step.UpdateTimeStep? {
+          SimpleStepPreservesInv(fs, fs', step);
+        }
+      }
+    }
+  }
 
-  // lemma DeletePreservesInv(fs: FileSys, fs': FileSys, path: Path, ctime: Time)
-  // requires Inv(fs)
-  // requires Delete(fs, fs', path, ctime)
-  // ensures Inv(fs')
-  // {
-  //   forall p | PathExists(fs', p) && p != RootDir
-  //   ensures ParentDirIsDir(fs', p)
-  //   {
-  //     assert PathExists(fs, p); // observe
-  //   }
+  lemma DeletePreservesInv(fs: FileSys, fs': FileSys, path: Path, ctime: Time)
+  requires Inv(fs)
+  requires Delete(fs, fs', path, ctime)
+  ensures Inv(fs')
+  {
+    forall p | PathExists(fs', p) && p != RootDir
+    ensures ParentDirIsDir(fs', p)
+    {
+      assert PathExists(fs, p); // observe
+    }
 
-  //   // forall p | fs'.meta_map[p].RedirectMeta? 
-  //   // ensures fs'.meta_map[fs'.meta_map[p].source].PathMeta?
-  //   // ensures fs'.meta_map[fs'.meta_map[p].source].hidden
-  //   // ensures !fs'.meta_map[fs'.meta_map[p].source].m.ftype.Directory?
-  //   // {
-  //   //   var m := fs.meta_map[path];
+    forall hidden | fs'.hidden.meta_map[hidden].MetaData?
+    ensures HasReference(fs', hidden)
+    {
+      var p :| fs.content.meta_map[p] == RedirectMeta(hidden) && p != path;
+      assert fs'.content.meta_map[p] == fs.content.meta_map[p]; // observe
+    }
 
-  //   //   if m.RedirectMeta? && fs'.meta_map[p].source == m.source {
-  //   //     assert fs.meta_map[p] == fs'.meta_map[p];
-  //   //     assert fs'.meta_map[m.source] == MetaDataDelete(fs, path, ctime);
+    assert Inv(fs');
+  }
 
-  //   //     if NoAlias(fs, path) {
-  //   //       assert p != path;
-  //   //       assert false;
-  //   //     }
-  //   //   }
-  //   // }
-  //   assert Inv(fs');
-  // }
+  lemma NoValidBeneathDir(fs: FileSys, dir: Path, path: Path)
+  requires Inv(fs)
+  requires BeneathDir(dir, path)
+  requires && fs.content.meta_map[dir].MetaData? 
+           && fs.content.meta_map[dir].ftype.Directory? ==> IsEmptyDir(fs, dir)
+  ensures !PathExists(fs, path)
+  {
+    var pdir := GetParentDir(path);
+    if pdir != dir {
+      NoValidBeneathDir(fs, dir, pdir);
+    }
+  }
 
-  // // lemma RenamedPathsRemainDifferent(src: Path, dst: Path, p1: Path, p2: Path)
-  // // requires p1 != p2
-  // // requires p1 == dst || BeneathDir(dst, p1)
-  // // requires p2 == dst || BeneathDir(dst, p2)
-  // // ensures src + p1[|dst|..] != src + p2[|dst|..]
-  // // {
-  // //   if BeneathDir(dst, p1) && BeneathDir(dst, p2) {
-  // //     assert p1[|dst|..] != p2[|dst|..];
+  lemma RenamePreservesInv(fs: FileSys, fs': FileSys, src: Path, dst: Path, ctime: Time)
+  requires Inv(fs)
+  requires Rename(fs, fs', src, dst, ctime)
+  ensures Inv(fs')
+  {
+    forall p | PathExists(fs', p) && p != RootDir
+    ensures ParentDirIsDir(fs', p)
+    {
+      if p == dst {
+        assert ParentDirIsDir(fs', dst);
+      } else if BeneathDir(dst, p) {
+        var parent_dir := GetParentDir(p);
+        var srcpath := src + p[|dst|..];
+        assert ParentDirIsDir(fs, srcpath); // observe
+        assert src + parent_dir[|dst|..] == GetParentDir(srcpath); // observe
+        assert ParentDirIsDir(fs', p);
+      } else {
+        assert PathExists(fs, p); // observe
+      }
+    }
 
-  // //     var p1' := src + p1[|dst|..];
-  // //     var p2' := src + p2[|dst|..];
+    forall p | fs'.content.meta_map[p].RedirectMeta?
+    ensures ValidHiddenEntry(fs', p)
+    {
+      if fs.content.meta_map[dst].RedirectMeta? && BeneathDir(dst, p) {
+        var srcpath := src + p[|dst|..];
+        assert fs'.content.meta_map[p] == fs.content.meta_map[srcpath];
+      }
+    }
 
-  // //     assert p1'[..|src|] == p2'[..|src|];
-  // //   }
-  // // }
+    forall hidden | fs'.hidden.meta_map[hidden].MetaData?
+    ensures HasReference(fs', hidden)
+    {
+      var p :| fs.content.meta_map[p] == RedirectMeta(hidden);
+      if p == src {
+        assert fs'.content.meta_map[dst] == RedirectMeta(hidden); // observe
+      } else if BeneathDir(src, p) {
+        var p' := dst + p[|src|..];
+        assert src + p'[|dst|..] == p; // observe
+        assert fs'.content.meta_map[p'] == fs.content.meta_map[p]; // observe
+      } else if p == dst {
+        var alias :| fs.content.meta_map[alias] == RedirectMeta(hidden) && alias != dst;
+        if BeneathDir(src, alias) {
+          NoValidBeneathDir(fs, src, alias);
+        }
+        if BeneathDir(dst, alias) {
+          NoValidBeneathDir(fs, dst, alias);
+        }
+        assert fs'.content.meta_map[alias] == fs.content.meta_map[alias];
+      } else if BeneathDir(dst, p) {
+        NoValidBeneathDir(fs, dst, p);
+      } else if p == GetParentDir(src) || p == GetParentDir(dst) {
+        assert HasReference(fs', hidden); 
+      } else {
+        assert fs'.content.meta_map[p] == fs.content.meta_map[p];
+        assert HasReference(fs', hidden);
+      }
+    }
 
-  // lemma RenamePreservesInv(fs: FileSys, fs': FileSys, src: Path, dst: Path, ctime: Time)
-  // requires Inv(fs)
-  // requires Rename(fs, fs', src, dst, ctime)
-  // ensures Inv(fs')
-  // {
-  //   forall p | PathExists(fs', p) && p != RootDir
-  //   ensures ParentDirIsDir(fs', p)
-  //   {
-  //     if p == dst {
-  //       assert fs'.meta_map[p] == UpdatePathCtime(fs, src, ctime);
-  //       assert ParentDirIsDir(fs', dst);
-  //       // if PathExists(fs, dst) {
-  //       //   assert ParentDirIsDir(fs, dst);
-  //       //   assert ParentDirIsDir(fs', dst);
-  //       // } else {
-  //       //   assert ValidNewPath(fs, dst);
-  //       //   assert ParentDirIsDir(fs, dst);
-  //       //   assert GetParentDir(dst) != dst;
-  //       //   assert GetParentDir(src) != src;
-  //       //   assert fs'.meta_map[GetParentDir(dst)] == UpdatePathTime(fs, GetParentDir(dst), ctime);
-  //       //   assert ParentDirIsDir(fs', dst); // why?
-  //       // }
-  //       // assert ParentDirIsDir(fs', p);
-  //     } else if BeneathDir(dst, p) {
-  //       var srcpath := src + p[|dst|..];
-  //       assert PathExists(fs, srcpath);
+    assert Inv(fs');
+  }
 
+  lemma LinkPreservesInv(fs: FileSys, fs': FileSys, source: Path, dest: Path, ctime: Time, hiddenName: Option<Path>)
+  requires Inv(fs)
+  requires Link(fs, fs', source, dest, ctime, hiddenName)
+  ensures Inv(fs')
+  {
+    forall p | PathExists(fs', p) && p != RootDir
+    ensures ParentDirIsDir(fs', p)
+    {
+      if p != dest {
+        assert PathExists(fs, p); // observe
+      }
+    }
 
-  //       // var parent_dir := GetParentDir(p);
-  //       //
-  //       // assert ParentDirIsDir(fs, srcpath); // observe
-  //       // assert src + parent_dir[|dst|..] == GetParentDir(srcpath); // observe
-  //       // assert parent_dir == dst || BeneathDir(dst, parent_dir); // observe
-  //       // assert fs'.meta_map[dst] == UpdatePathCtime(fs, src, ctime); // observe
+    forall hidden | fs'.hidden.meta_map[hidden].MetaData?
+    ensures HasReference(fs', hidden)
+    {
+      if hiddenName.Some? && hiddenName.value == hidden {
+        assert fs'.content.meta_map[source] == RedirectMeta(hidden); // observe
+      } else {
+        var p :| fs.content.meta_map[p] == RedirectMeta(hidden);
+        assert fs'.content.meta_map[p] == fs.content.meta_map[p]; // observe
+      }
+    }
 
+    assert Inv(fs');
+  }
 
-  //       assume ParentDirIsDir(fs', p);
+  lemma SimpleStepPreservesInv(fs: FileSys, fs': FileSys, step: Step)
+  requires Inv(fs)
+  requires NextStep(fs, fs', step)
+  requires step.CreateStep? || step.ChangeAttrStep? || step.TruncateStep? || step.WriteStep? || step.UpdateTimeStep?
+  ensures Inv(fs')
+  {
+    forall p | PathExists(fs', p) && p != RootDir 
+    ensures ParentDirIsDir(fs', p)
+    {
+      if p != step.path {
+        assert PathExists(fs, p); // observe
+      }
+    }
 
-  //     } else {
-  //       assert PathExists(fs, p); // observe
-  //       // assert ParentDirIsDir(fs, p); // observe
-  //       // assert ParentDirIsDir(fs', p);
-  //     }
-  //   }
+    forall hidden | fs'.hidden.meta_map[hidden].MetaData?
+    ensures HasReference(fs', hidden)
+    {
+      var p :| fs.content.meta_map[p] == RedirectMeta(hidden);
+      assert fs'.content.meta_map[p] == fs.content.meta_map[p]; // observe
+    }
 
-
-
-  //   // forall p | PathExists(fs', p) && p != RootDir
-  //   // ensures ParentDirIsDir(fs', p)
-  //   // {
-  //   //   if p == dst {
-  //   //     assert fs'.meta_map[p] == UpdatePathCtime(fs, src, ctime);
-  //   //     assert ParentDirIsDir(fs', dst);
-  //   //     // if PathExists(fs, dst) {
-  //   //     //   assert ParentDirIsDir(fs, dst);
-  //   //     //   assert ParentDirIsDir(fs', dst);
-  //   //     // } else {
-  //   //     //   assert ValidNewPath(fs, dst);
-  //   //     //   assert ParentDirIsDir(fs, dst);
-  //   //     //   assert GetParentDir(dst) != dst;
-  //   //     //   assert GetParentDir(src) != src;
-  //   //     //   assert fs'.meta_map[GetParentDir(dst)] == UpdatePathTime(fs, GetParentDir(dst), ctime);
-  //   //     //   assert ParentDirIsDir(fs', dst); // why?
-  //   //     // }
-  //   //     // assert ParentDirIsDir(fs', p);
-  //   //   } else if BeneathDir(dst, p) {
-  //   //     var srcpath := src + p[|dst|..];
-  //   //     assert PathExists(fs, srcpath);
-
-
-  //   //     // var parent_dir := GetParentDir(p);
-  //   //     //
-  //   //     // assert ParentDirIsDir(fs, srcpath); // observe
-  //   //     // assert src + parent_dir[|dst|..] == GetParentDir(srcpath); // observe
-  //   //     // assert parent_dir == dst || BeneathDir(dst, parent_dir); // observe
-  //   //     // assert fs'.meta_map[dst] == UpdatePathCtime(fs, src, ctime); // observe
-
-
-  //   //     assume ParentDirIsDir(fs', p);
-
-  //   //   } else {
-  //   //     assert PathExists(fs, p); // observe
-  //   //     // assert ParentDirIsDir(fs, p); // observe
-  //   //     // assert ParentDirIsDir(fs', p);
-  //   //   }
-  //   // }
-
-  //   forall p | fs'.meta_map[p].RedirectMeta? 
-  //   ensures fs'.meta_map[fs'.meta_map[p].source].PathMeta?
-  //   ensures fs'.meta_map[fs'.meta_map[p].source].hidden
-  //   ensures !fs'.meta_map[fs'.meta_map[p].source].m.ftype.Directory?
-  //   {
-  //     // assert p != dst;
-  //     // assert p != src && !BeneathDir(src, p);
-
-  //     assume false;
-
-  //     // spec should skip hidden ones when moving things right?
-  //     // otherwise we would be 
-
-  //     // maybe we should have something that says we don't move the hidden name 
-
-
-  //     // if fs.meta_map[dst].RedirectMeta? && fs.meta_map[dst].source == p {
-  //     //   assume false;
-  //     // } else if p == GetParentDir(src) || p == GetParentDir(dst) {
-  //     //   // assume false;
-  //     // } else {
-
-  //     //   assume false;
-  //     // }
-
-  //     // imap path ::
-  //     // if path == src || BeneathDir(src, path) then Empty
-  //     // else if path == dst then UpdatePathCtime(fs, src, ctime)
-  //     // else if BeneathDir(dst, path) then (
-  //     //   var suffix := path[|dst|..];
-  //     //   fs.meta_map[src + suffix]
-  //     // ) else 
-      
-  //     // if fs.meta_map[dst].RedirectMeta? && fs.meta_map[dst].source == path then (
-  //     //   UpdatePathCtime(fs, dst, ctime)
-  //     // ) else if path == GetParentDir(src) || path == GetParentDir(dst) then (
-  //     //   UpdatePathTime(fs, path, ctime)
-  //     // ) else (
-  //     //   fs.meta_map[path]
-  //     // )
-
-  //     // assume false;
-  //     // if (p == dest || p == source) && fs.meta_map[source].PathMeta? {
-  //     //   assert fs'.meta_map[hiddenName.value] == LinkMeta(fs, source, ctime);
-  //     // }
-  //   }
-  //   assert Inv(fs');
-  // }
-
-  // lemma LinkPreservesInv(fs: FileSys, fs': FileSys, source: Path, dest: Path, ctime: Time, hiddenName: Option<Path>)
-  // requires Inv(fs)
-  // requires Link(fs, fs', source, dest, ctime, hiddenName)
-  // ensures Inv(fs')
-  // {
-  //   forall p | PathExists(fs', p) && p != RootDir
-  //   ensures ParentDirIsDir(fs', p)
-  //   {
-  //     if p == dest {
-  //       assert ParentDirIsDir(fs', p);
-  //     } else {
-  //       assert PathExists(fs, p); // observe
-  //     }
-  //   }
-
-  //   forall p | fs'.meta_map[p].RedirectMeta? 
-  //   ensures fs'.meta_map[fs'.meta_map[p].source].PathMeta?
-  //   ensures fs'.meta_map[fs'.meta_map[p].source].hidden
-  //   ensures !fs'.meta_map[fs'.meta_map[p].source].m.ftype.Directory?
-  //   {
-  //     if (p == dest || p == source) && fs.meta_map[source].PathMeta? {
-  //       assert fs'.meta_map[hiddenName.value] == LinkMeta(fs, source, ctime);
-  //     }
-  //   }
-  //   assert Inv(fs');
-  // }
-
-  // lemma SimpleStepPreservesInv(fs: FileSys, fs': FileSys, step: Step)
-  // requires Inv(fs)
-  // requires NextStep(fs, fs', step)
-  // requires step.CreateStep? || step.ChangeAttrStep? || step.TruncateStep? || step.WriteStep? || step.UpdateTimeStep?
-  // ensures Inv(fs')
-  // {
-  //   forall p | PathExists(fs', p) && p != RootDir 
-  //   ensures ParentDirIsDir(fs', p)
-  //   {
-  //     if p != step.path {
-  //       assert PathExists(fs, p); // observe
-  //     }
-  //   }
-  //   assert Inv(fs');
-  // }
+    assert Inv(fs');
+  }
 }
